instnat_mod.

PsBool.v
@@ -1,9 +1,5 @@
-Require Import Basics.
-Require Import Relations.
-Require Import List.
-
-Require Import Utils.
-Require Import PsCore.
+Require Import Basics Relations List.
+Require Import Utils PsCore.
 
 Definition instfalse_spec (i1 : inst) : Prop :=
   forall (i2 i3 : inst) (vs ps : stack),
@@ -30,20 +26,26 @@ Qed.
 
 Definition instnot := instseq [ instpush ; instswap ; instcons ].
 
-Lemma instnot_proof : forall (b : bool) (i1 : inst) (vs ps : stack),
-  instbool_spec b i1 ->
-    exists i2 : inst,
-      instbool_spec (negb b) i2 /\
-      (i1 :: vs, instnot :: ps) |=>* (i2 :: vs, ps).
+Lemma instnot_proof :
+  forall (b : bool) (i1 : inst) (vs ps : stack), instbool_spec b i1 ->
+    exists i2 : inst, instbool_spec (negb b) i2 /\
+    (i1 :: vs, instnot :: ps) |=>* (i2 :: vs, ps).
   intros ; evalauto ; destruct b ;
     repeat intro ; evalauto ; evalpartial H ; evalauto.
 Qed.
 
-Definition instif := instseq [ instexec ; instswap ; instpop ].
+Opaque instnot.
+
+Definition instif := instseq
+  [ instquote ;
+    instswap ; instquote ; instsnoc ;
+    instswap ; instquote ; instcons ;
+    instexec ;
+    instexec ; instswap ; instpop ].
 
 Lemma eval_instif : forall (b : bool) (i1 i2 i3 : inst) (vs ps : stack),
-  instbool_spec b i3 -> (i3 :: i2 :: i1 :: vs, instif :: ps) |=>*
-    ((if b then i1 else i2) :: vs, ps).
+  instbool_spec b i1 -> (i3 :: i2 :: i1 :: vs, instif :: ps) |=>*
+    ((if b then i2 else i3) :: vs, ps).
   intros.
   destruct b ; evalauto ; evalpartial H ; evalauto.
 Qed.
@@ -51,8 +53,8 @@ Qed.
 Definition instexecif := instseq [ instif ; instexec ].
 
 Lemma eval_instexecif : forall (b : bool) (i1 i2 i3 : inst) (vs ps : stack),
-  instbool_spec b i3 -> (i3 :: i2 :: i1 :: vs, instexecif :: ps) |=>*
-    (vs, (if b then i1 else i2) :: ps).
+  instbool_spec b i1 -> (i3 :: i2 :: i1 :: vs, instexecif :: ps) |=>*
+    (vs, (if b then i2 else i3) :: ps).
   intros.
   destruct b ; evalauto ; evalpartial H ; evalauto.
 Qed.
@@ -61,9 +63,10 @@ Definition instxor := instcons.
 
 Lemma instxor_proof : forall (b1 b2 : bool) (i1 i2 : inst) (vs ps : stack),
   instbool_spec b1 i1 -> instbool_spec b2 i2 ->
-    exists i3 : inst,
-      instbool_spec (xorb b1 b2) i3 /\
-      (i2 :: i1 :: vs, instxor :: ps) |=>* (i3 :: vs, ps).
+    exists i3 : inst, instbool_spec (xorb b1 b2) i3 /\
+    (i2 :: i1 :: vs, instxor :: ps) |=>* (i3 :: vs, ps).
   intros ; evalauto ; destruct b1, b2 ; repeat intro ;
     evalauto ; evalpartial H ; evalpartial H0 ; evalauto.
 Qed.
+
+Opaque instxor.
